Queue proof

examples/Queue.v
@@ -6,6 +6,7 @@ From CTree Require Import
   Logic.Kripke
   CTree.Interp.Core
   CTree.Logic.AF
+  CTree.Logic.AX
   CTree.Logic.CanStep
   CTree.Interp.State
   CTree.Events.State
@@ -45,9 +46,12 @@ Definition push {S}: S -> ctree (queueE S) unit :=
 Definition pop {S}: ctree (queueE S) (option S) :=
   Ctree.trigger Pop.
 
+Arguments push /.
+Arguments pop /.
+
 Section QueueEx.
   Context {S: Type}.
-  (* Drain a queue *)
+  (* Ex1: Drain a queue *)
   Definition drain: ctree (queueE S) unit :=
     iter (fun _ =>
             x <- pop ;;
@@ -56,26 +60,38 @@ Section QueueEx.
             | None => Ret (inr tt)   (* done *)
             end) tt.
 
-  Global Instance handler_queueE: queueE S ~> state (list S) := {
-      handler e :=
-        mkState (fun q =>
-                   match e return encode e * list S with
-                   | Push v => (tt, q ++ [v])
-                   | Pop => match q with
-                           | nil => (None, nil)
-                           | h :: ts => (Some h, ts)
-                           end
-                   end)
-    }.
+  (* Ex2: Rotate (pop an element, add an element [a]) a queue (a ≠ b) *)
+  Definition rotate(a: S): ctree (queueE S) unit :=
+    iter (fun _ =>
+            push a ;;
+            x <- pop ;;
+            match x with
+            | Some v => Ret (inl tt)
+            | None => Ret (inr tt) (* should never return *)
+            end) tt.            
+      
+  Definition h_queueE: queueE S ~> state (list S) := 
+    fun e =>
+      mkState (fun q =>
+                 match e return encode e * list S with
+                 | Push v => (tt, q ++ [v])
+                 | Pop => match q with
+                         | nil => (None, nil)
+                         | h :: ts => (Some h, ts)
+                         end
+                 end).
 
-  (* Pick this view of the system, the semantics are [handler_queueE] *)
+  (* Pick this view of the queue to instrument *)
   Variant view :=
     | VPop (queue: list S) (elem: S)
     | VPush (queue: list S) (elem: S)
     | VEmpty.
 
   Definition instr_queueE: queueE S ~> stateT (list S) (ctree (writerE view)) :=
-    h_writerA _
+    h_writerA
+      (* queue semantics *)
+      (h_state h_queueE)
+      (* queue instrumentation *)
       (fun (e: queueE S) (v: encode e) (q: list S) =>
          match e return encode e -> view with
          | Pop => fun x: option S =>
@@ -86,10 +102,10 @@ Section QueueEx.
          | Push x => fun _ => VPop q x
          end v).
 
-  Print writerE.
+
   (*| Eventually we get [s] |*)
-  Check finish_with.
-  Theorem ctl_queue_eventually: forall (s: S) q,
+  Typeclasses Transparent equ.
+  Theorem drain_af_pop: forall (s: S) q,
       <( {interp_state instr_queueE drain (q ++ [s])}, Pure |=
          AF finish {fun '(Log v) 'tt 'tt => v = VPop nil s } )>.
   Proof.
@@ -99,84 +115,35 @@ Section QueueEx.
     revert s.
     induction q; intros. 
     - setoid_rewrite interp_state_unfold_iter.
-      Check af_bind_r.
-      Print finish_with.
-      eapply af_bind_r.
-      + unfold pop.
-        Check @bind_trigger.
-        replace (x <- trigger Pop;; match x with
-                                   | Some _ => Ret (inl tt)
-                                   | None => Ret (inr tt)
-                                   end) with (x <- trigger Pop;; match x with
-                                   | Some _ => Ret (inl tt)
-                                   | None => Ret (inr tt)
-                                                                end
-                                                                  match (Some s: option S) with
-                                              | Some _ => Ret (inl tt)
-                                              | None => Ret (inr tt)
-                                              end).
-        setoid_rewrite bind_trigger.
-        unfold pop, trigger.
-        rewrite bind_vis.
+      eapply af_bind_r_eq.
+      + rewrite interp_state_bind.
+        rewrite List.app_nil_l.        
+        unfold pop, trigger, resum, ReSum_refl.
         rewrite interp_state_vis.
         cbn.
-        setoid_rewrite bind_bind.
-        unfold pop.
-        rewrite resumCtree_Ret.
-
-      setoid_rewrite bind_trigger.
-      eapply ctl_bind_af_l.
-      next; right.
-      next; split.
-      + econstructor. setoid_rewrite ktrans_vis; eauto.
-      + intros [t' w'] TR.
-        apply ktrans_vis in TR as (? & ? & ?).
-        rewrite <- H, H0.
-        apply ctl_af_ax; left.
-        apply ctl_now; cbn.
-        eauto.
-    - setoid_rewrite interp_state_unfold_iter.
-      setoid_rewrite interp_state_bind.
-      setoid_rewrite bind_bind.
-      unfold pop, trigger.
-      setoid_rewrite interp_state_vis.
-      cbn.
-      rewrite !bind_bind.
-      eapply ctl_bind_af_r; [cbn; econstructor|].
-      cbn.
-      setoid_rewrite bind_trigger.
-      setoid_rewrite bind_vis.
-      next; right.
-      next; split.
-      + cbn; econstructor.
-        eexists.
-        apply ktrans_vis; eauto.
-      + intros [t' w'] TR.
-        apply ktrans_vis in TR as (? & ? & ?).
-        rewrite <- H, H0; clear H H0.
-        rewrite bind_ret_l, bind_guard.
-        rewrite <- ctl_guard_af.
-        setoid_rewrite interp_state_ret.
-        unfold resum_ret, ReSumRet_refl; cbn.
+        repeat rewrite bind_bind.
+        resum.
         rewrite bind_ret_l.
-        setoid_rewrite interp_state_ret.
-        rewrite bind_ret_l.
-        rewrite <- !ctl_guard_af.
-        apply IHq.
-        Unshelve.
-        exact tt.
-        exact tt.
-  Qed.
-
-  (* Rotate a queue of bools (pop/push) *)
-  Definition rotate: ctree (queueE bool) unit :=
-    forever (fun _ =>
-               x <- pop ;;
-               if x then
-                 push true
-               else
-                 push false
-      ) tt.
+        rewrite bind_trigger, bind_vis.
+        unfold resum, ReSum_refl.
+        next; right.
+        next; split; eauto with ctl.
+        * apply can_step_vis; auto with ctl.
+        * intros t' w' TR.
+          apply ktrans_vis in TR as (x & -> & Heqt & Hd).
+          rewrite bind_ret_l in Heqt.
+          rewrite bind_tau in Heqt.
+          rewrite <- Heqt.
+          next; left.
+          apply ax_tau.          
+          rewrite interp_state_ret.
+          rewrite bind_ret_l.
+          cbn.          
+          rewrite interp_state_ret.
+          apply ax_finish; split; destruct x; eauto.
+      + cbn.
+        apply af_tau.
+  Admitted.
 
   (*
   forever p x |= AF now φ
@@ -184,16 +151,12 @@ Section QueueEx.
   forever p x |= WG WF now φ
    *)
   
-  (*| Always eventually we get [true] |*)
-  Theorem ctl_rotate_always_eventually: forall (s: bool) q x,
-      <( {(interp_state instr_queueE rotate (q ++ [true]), x)} |=
-         AG AF now {fun '(Obs (Log e) _) => pops_s e true} )>.
+  (*| Even though [rotate] does not terminate, we eventually get [a] |*)
+  Theorem rotate_af_pop: forall (a b: S) (Hneq: a <> b) q w,
+      <( {interp_state instr_queueE (rotate b) (q ++ [a])}, w |=
+         AF vis {fun '(Log v) 'tt => exists l, v = VPop l a})>.
   Proof.
     intros.
-    revert s x.
-    induction q; intros.
-    - unfold rotate.
-      setoid_rewrite app_nil_l.
   Admitted.
 End QueueEx.
   
