theories/ITree/Interp.v
@@ -8,6 +8,7 @@ From CTree Require Import
   ITree.Core
   ITree.Equ.
 
+Generalizable All Variables.
 Set Implicit Arguments.
 
 Import MonadNotation.
@@ -17,13 +18,13 @@ Open Scope monad_scope.
 (** An event handler [E ~> M] defines a monad morphism
     [ctree E ~> M] for any monad [M] with a loop operator. *)
 
-Definition interp {E} {M : Type -> Type}
+Definition interp `{Encode E} {M : Type -> Type}
   {MM : Monad M} {MI : MonadIter M} (h: E ~> M) : forall X, itree E X -> M X :=
   fun R => iter (fun t =>
                 match observe t with
                 | RetF r => ret (inr r)
                 | TauF t => ret (inl t)
-                | VisF e k => x <- h.(handler) e ;; ret (inl (k x))
+                | VisF e k => x <- h e ;; ret (inl (k x))
                 end).
 
-Arguments interp {E M MM MI} h [X].
+Arguments interp {E H M MM MI} h [X].
