theories/Events/Core.v
@@ -24,53 +24,54 @@ Arguments encode: simpl never.
           | inl e1 => encode e1
           | inr e2 => encode e2 end.
 
+(** Typeclasses designed to implement a subevent relation, relied on by the trigger function *)
+Class ReSum (E1 E2 : Type@{eff}) : Type := resum : E1 -> E2.
+Class ReSumRet E1 E2 `{Encode E1} `{Encode E2} `{ReSum E1 E2} : Type :=
+  resum_ret : forall (e : E1), encode (resum e) -> encode e.
+
+#[global] Instance ReSum_inl {E1 E2} : ReSum E1 (E1 + E2) :=
+  inl.
+#[global] Instance ReSum_inr {E1 E2} : ReSum E2 (E1 + E2) :=
+  inr.
+
+#[global] Instance ReSumRet_inl {E1 E2} `{Encode E1} `{Encode E2}: ReSumRet E1 (E1 + E2) := fun _ e => e.
+
+#[global] Instance ReSumRet_inr {E1 E2} `{Encode E1} `{Encode E2} : ReSumRet E2 (E1 + E2) := fun _ e => e.
+
+#[global] Instance ReSum_refl {E} : ReSum E E :=
+  fun e => e.
+#[global] Instance ReSumRet_refl {E} `{Encode E}:
+  ReSumRet E E := fun _ e => e.
+
 (*| Empty effect |*)
 Variant void: Type :=.
 
 #[global] Instance encode_void: Encode void :=
   fun e => match e with end.
 
-(** Typeclasses designed to implement a subevent relation, relied on by the trigger function *)
-Class ReSum (E1 E2 : Type@{eff}) : Type := resum : E1 -> E2.
-Class ReSumRet E1 E2 `{Encode E1} `{Encode E2} `{ReSum E1 E2} : Type :=
-  resum_ret : forall (e : E1), encode (resum e) -> encode e.
+#[global] Instance ReSum_void {E} : ReSum void E :=
+  fun e => match e with end.
 
-#[global] Instance ReSum_inl {E1 E2} : ReSum E1 (E1 + E2) := inl.
-#[global] Instance ReSum_inr {E1 E2} : ReSum E2 (E1 + E2) := inr.
+#[global] Instance ReSumRet_void {E} `{Encode E} :
+  ReSumRet void E := fun e _ => match e with end. 
 
-#[global] Instance ReSumRet_inl {E1 E2} `{Encode E1} `{Encode E2}: ReSumRet E1 (E1 + E2) :=
-  fun _ e => e.
-#[global] Instance ReSumRet_inr {E1 E2} `{Encode E1} `{Encode E2} : ReSumRet E2 (E1 + E2) :=
-  fun _ e => e.
-
-#[global] Instance ReSum_void {E} : ReSum void E := fun e => match e with end.
-
-#[global] Instance ReSumRet_void {E} `{Encode E}: ReSumRet void E :=
-  fun e _ => match e with end. 
-
-#[global] Instance ReSum_refl {E} : ReSum E E := fun e => e.
-#[global] Instance ReSumRet_refl {E} `{Encode E}: ReSumRet E E :=
-  fun _ e => e.
-
-(*| Defines a monad homomorphism from free monad with [E] to [M] |*)
-Class Handler(E: Type) (M: Type -> Type): Type := {
-    #[global] Handler_Encode :: Encode E;
-    handler(e: E) : M (encode e)
-  }.
+(*| Defines a monad homomorphism from free monad with [E]
+  to monad [M] |*)
+Definition Handler E M `{Encode E} `{Monad M}: Type :=
+  forall (e: E), M (encode e).
 
 Notation "E ~> M" := (Handler E M) (at level 68, right associativity). 
 
-#[global] Instance handler_exfalso `{Monad M} {Σ : Type} : void ~> M  := {
-    handler(e : void) := match e with end
-  }.
+Definition h_void `{Monad M}: void ~> M :=
+  fun (e : void) => match e with end.
 
-#[global] Instance handler_plus{A B} `{Monad M} `{CA: A ~> M} `{CB: B ~> M}: A + B ~> M := {
-    handler e :=
-      match e with
-      | inl e => handler e
-      | inr e => handler e
-      end
-  }.
+Definition h_sum{A B} `{Monad M} `{Encode A} `{Encode B}
+  (ha: A ~> M) (hb: B ~> M):
+  A + B ~> M := fun e =>
+                  match e with
+                  | inl e => ha e
+                  | inr e => hb e
+                  end.
 
 (*| Dependent observations require dependent equality |*)
 Definition eq_dep_obs`{Encode E} {e e':E}(v: encode e)(v': encode e'): Prop :=
